Proved several diagram-cases for eq. Case eq-inject seems to need additional axiom on coresemantics:   corestep c m c' m' -> mem_forward m m'. Indeed, there's a similar condition on external calls in Events.v,   so the fact that we appear to need the axiom is not too surprising. Spoiler alert: similar axioms will presumably be required for   some/all of the other axioms in Events.v.

veric/CC_trans.v
@@ -3,6 +3,34 @@ Require Import veric.base.
 Require Import compcert.Events.
 Require Import veric.sim.
 Require Import veric.MemoryPushouts.
+Require Import Wellfounded.
+
+(*It seems we need the following property to be satisfied by at least Sem2 and Sem3.
+  Probably we should add it as an axiom to CoreSemantics in sim.v.
+  The fact that this property is required should not be too surprising: it corresponds to
+  the axiom ec_valid_blockin Events.v*)
+Definition corestep_fwd {G C D} (Sem: CoreSemantics G C mem D) :=
+forall g c m c' m' (CS: corestep Sem g c m c' m'), mem_forward m m'.
+
+Lemma corestepN_fwd: forall {G C D} (Sem: CoreSemantics G C mem D)
+              (Fwd: corestep_fwd Sem) g N c m c' m' (CS:corestepN Sem g N c m c' m'), 
+               mem_forward m m'.
+Proof. intros G C D Sem Fwd g N.
+  induction N; simpl; intros.
+       inv CS. apply mem_forward_refl. 
+       destruct CS as [c2 [m2 [CS1 CS2]]].
+           apply Fwd in CS1. apply IHN in CS2. eapply mem_forward_trans; eassumption.
+Qed. 
+
+Lemma corestep_star_fwd: forall {G C D} (Sem: CoreSemantics G C mem D)
+              (Fwd: corestep_fwd Sem) g c m c' m' (CS:corestep_star Sem g c m c' m'), 
+               mem_forward m m'.
+Proof. intros. destruct CS.  eapply  corestepN_fwd. apply Fwd. apply H. Qed.
+
+Lemma corestep_plus_fwd: forall {G C D} (Sem: CoreSemantics G C mem D)
+              (Fwd: corestep_fwd Sem) g c m c' m' (CS:corestep_plus Sem g c m c' m'), 
+               mem_forward m m'.
+Proof. intros. destruct CS.  eapply  corestepN_fwd. apply Fwd. apply H. Qed.
 
 Definition main_sig : signature := 
        mksignature (nil) (Some AST.Tint).
@@ -10,47 +38,15 @@ Definition main_sig : signature :=
 Definition entrypoints_compose (ep12 ep23 ep13 : list (val * val * signature)): Prop :=
    forall v1 v3 sig, In (v1,v3,sig) ep13 = exists v2, In (v1,v2,sig) ep12 /\ In (v2,v3,sig) ep23.
 
-Lemma cc_trans_CaseEq: forall {F1 C1 V1 F2 C2 V2 F3 C3 V3} 
-     (Sem1 : CoreSemantics (Genv.t F1 V1) C1 mem (list (ident * globvar V1)))
-     (Sem2 : CoreSemantics (Genv.t F2 V2) C2 mem (list (ident * globvar V2)))
-     (Sem3 : CoreSemantics (Genv.t F3 V3) C3 mem (list (ident * globvar V3)))
-     ExternIdents epts12 epts23 I 
-     (P1 : AST.program F1 V1) (P2 : AST.program F2 V2) (P3 : AST.program F3 V3)
-     (ePts12_ok : CompilerCorrectness.entryPts_ok P1 P2 ExternIdents epts12)
-     (e12 : prog_main P1 = prog_main P2)
-     (g12: CompilerCorrectness.GenvHyp P1 P2)
-     (Eq_init12 : forall m1 : mem,
-          initial_mem Sem1 (Genv.globalenv P1) m1 (prog_vars P1) ->
-          exists m2 : mem,
-            initial_mem Sem2 (Genv.globalenv P2) m2 (prog_vars P2) /\ m1 = m2)
-     (SimEq12 : Sim_eq.Forward_simulation_equals mem (list (ident * globvar V1))
-                                (list (ident * globvar V2)) Sem1 Sem2 (Genv.globalenv P1)
-                               (Genv.globalenv P2) epts12)
-     (SIM23 : CompilerCorrectness.cc_sim I ExternIdents epts23 F2 C2 V2 F3 C3 V3 Sem2 Sem3 P2 P3)
-     (i1: I F1 C1 V1 Sem1 P1),
-forall entrypoints13 : list (val * val * signature),
-entrypoints_compose epts12 epts23 entrypoints13 ->
-In (prog_main P1, CompilerCorrectness.extern_func main_sig) ExternIdents ->
-prog_main P1 = prog_main P2 ->
-In (prog_main P2, CompilerCorrectness.extern_func main_sig) ExternIdents ->
-prog_main P2 = prog_main P3 ->
-CompilerCorrectness.cc_sim I ExternIdents entrypoints13 F1 C1 V1 F3 C3 V3
-  Sem1 Sem3 P1 P3.
-Proof. 
-intros F1 C1 V1 F2 C2 V2 F3 C3 V3 Sem1 Sem2 Sem3 ExternIdents epts12 epts23 I  
-          P1 P2 P3 ePts12_ok e12 g12 Eq_init12 SimEq12 SIM23 i1.
-induction SIM23; intros; subst.
-     (*equality pass Sem2 -> Sem3*)  
-        rename C2 into C3. rename V2 into V3. rename F2 into F3. rename P2 into P3. rename Sem2 into Sem3.
-        rename C0 into C2. rename V0 into V2. rename F0 into F2. rename P0 into P2. rename Sem0 into Sem2.
-        clear H1 H3. rename Eq_init into Eq_init23. rename e into e23. rename g into g23. rename R into SimEq23.
-                               rename H0 into Extern1. rename H2 into Extern2. rename ePts_ok into ePts23_ok. rename H into EPC.
-                                rename i into i2. rename i0 into i3.
-       apply CompilerCorrectness.ccs_eq with (entrypoints:=entrypoints13); try assumption.
-         intros m1 Ini1.
-           destruct (Eq_init12 _ Ini1) as [m2 [Ini2 XX]]. subst.
-           apply (Eq_init23 _ Ini2).
-         unfold CompilerCorrectness.entryPts_ok; intros e d EXT.
+Lemma ePts_compose1: forall {F1 V1 F2 V2 F3 V3} 
+     (Prg1 : AST.program F1 V1) (Prg2 : AST.program F2 V2)  (Prg3 : AST.program F3 V3)
+     Epts12 Epts23 ExternIdents entrypoints13 
+    (EPC : entrypoints_compose Epts12 Epts23 entrypoints13)
+    (ePts12_ok : @CompilerCorrectness.entryPts_ok F1 V1 F2 V2 Prg1 Prg2 ExternIdents Epts12)
+    (ePts23_ok : @CompilerCorrectness.entryPts_ok F2 V2 F3 V3 Prg2 Prg3 ExternIdents Epts23),
+CompilerCorrectness.entryPts_ok Prg1 Prg3 ExternIdents entrypoints13.
+Proof. intros.
+            unfold CompilerCorrectness.entryPts_ok; intros e d EXT.
             destruct (ePts12_ok _ _ EXT) as [b [Find_b1 [Find_bb2 Hb]]].
             exists b; split; trivial.
             destruct (ePts23_ok _ _ EXT) as [bb [Find_b2 [Find_b3 Hbb]]].
@@ -61,7 +57,7 @@ induction SIM23; intros; subst.
                   rewrite Hff2 in Hf2. inv Hf2.
                   split. rewrite (EPC (Vptr b Int.zero) (Vptr b Int.zero) s). exists  (Vptr b Int.zero). split; assumption.
                   exists f1. exists f3. split; assumption.
-         destruct Hb as [v1 [v2 [Hv1 [Hv2 GV12]]]].
+           destruct Hb as [v1 [v2 [Hv1 [Hv2 GV12]]]].
            destruct Hbb as [vv2 [v3 [Hvv2 [Hv3 GV23]]]].
            rewrite Hvv2 in Hv2. inv Hv2.
            exists v1. exists v3. split; trivial. split; trivial.
@@ -70,125 +66,16 @@ induction SIM23; intros; subst.
                 destruct v3; simpl in *. 
                 destruct GV12 as [? [? ?]].
                 rewrite  H. rewrite H0. rewrite H1. assumption.
-         destruct SimEq12 as [core_data12 match_core12 core_ord12 core_ord_wf12 core_diagram12 core_initial12 core_halted12 core_at_external12 core_after_external12].  
-           destruct SimEq23 as [core_data23 match_core23 core_ord23 core_ord_wf23 core_diagram23 core_initial23 core_halted23 core_at_external23 core_after_external23].
-           eapply Sim_eq.Build_Forward_simulation_equals with
-                 (core_data:= prod core_data12 core_data23)
-                 (match_core := fun d c1 c3 => match d with (d1,d2) => exists c2, match_core12 d1 c1 c2 /\ match_core23 d2 c2 c3 end).
-             eapply wf_lex_ord. apply core_ord_wf12. apply core_ord_wf23.
-             admit. (*core_diagram
-             intros c1 m1 c1' m1' CS1 [d12 d23] c3 [c2 [MC12 MC23]].
-                 destruct (core_diagram12 _ _ _ _ CS1 _ _ MC12) as [c2' [d12' [MC12' X]]].
-                 destruct X as [CS2 | CS2 ord12'].
-                     destruct (core_diagram23 _ _ _ _ H3*)
-             (*initial_core*)
-                  intros. rename v2 into v3. rewrite (EPC v1 v3 sig) in H. destruct H as [v2 [EP12 EP23]].
-                  destruct (core_initial12 _ _ _ EP12 _ H0) as [d12 [c1 [c2 [Ini1 [Ini2 MC12]]]]].
-                  destruct (core_initial23 _ _ _ EP23 _ H0) as [d23 [c22 [c3 [Ini22 [Ini3 MC23]]]]].
-                  rewrite Ini22 in Ini2. inv Ini2.
-                  exists (d12,d23). exists c1. exists c3. split; trivial. split; trivial. exists c2. split; trivial.
-             (*safely_halted*)
-                    intros. rename c2 into c3. destruct cd as [d12 d23]. destruct H as [c2 [MC12 MC23]].
-                    apply (core_halted12 _ _ _ _ MC12) in H0.
-                    apply (core_halted23 _ _ _ _ MC23) in H0. assumption.
-             (*atexternal*)
-                    intros. rename st2 into st3. destruct d as [d12 d23]. destruct H as [st2 [MC12 MC23]].
-                    apply (core_at_external12 _ _ _ _ _ _ MC12) in H0. destruct H0.
-                    apply (core_at_external23 _ _ _ _ _ _ MC23) in H. assumption.  
-             (*after_external*)
-                    intros. rename st2 into st3. destruct d as [d12 d23]. destruct H as [st2 [MC12 MC23]].
-                    destruct (core_at_external12 _ _ _ _ _ _ MC12 H0)  as [AtExt2 _].
-                    destruct (core_after_external12 _ _ _ _ _ _ _ MC12 H0 AtExt2 H2 H3) as [c1' [c2' [d12' [AftExt1 [AftExt2 MS12']]]]].
-                    destruct (core_after_external23 _ _ _ _ _ _ _ MC23 AtExt2 H1 H2 H3) as [c22' [c3' [d23' [AftExt22 [AftExt3 MS23']]]]].
-                    rewrite AftExt22 in AftExt2. inv AftExt2.
-                    exists c1'. exists c3'. exists (d12',d23'). split; trivial. split; trivial. exists c2'. split; trivial.
-             (*prog_main*)
-                   rewrite e12; assumption.
-             (*GenvHyp*) 
-                   destruct g23 as [Hyp2A Hyp2B].
-                   split; intros. rewrite Hyp2A. apply g12. 
-                                        rewrite Hyp2B. apply g12.
-     (*extension pass Sem2 -> Sem3*) 
-        rename C2 into C3. rename V2 into V3. rename F2 into F3. rename P2 into P3. rename Sem2 into Sem3.
-        rename C0 into C2. rename V0 into V2. rename F0 into F2. rename P0 into P2. rename Sem0 into Sem2.
-        clear H1 H3. rename Extends_init into Ext_init23. rename e into e23. rename g into g23. rename R into SimExt23.
-                               rename H0 into Extern1. rename H2 into Extern2. rename ePts_ok into ePts23_ok. rename H into EPC.
-                                rename i into i2. rename i0 into i3.
-       apply CompilerCorrectness.ccs_ext with (entrypoints:=entrypoints13); try assumption.
-         intros m1 Ini1.
-           destruct (Eq_init12 _ Ini1) as [m2 [Ini2 XX]]. subst.
-           apply (Ext_init23 _ Ini2).
-         unfold CompilerCorrectness.entryPts_ok; intros e d EXT.
-            destruct (ePts12_ok _ _ EXT) as [b [Find_b1 [Find_bb2 Hb]]].
-            exists b; split; trivial.
-            destruct (ePts23_ok _ _ EXT) as [bb [Find_b2 [Find_b3 Hbb]]].
-            rewrite Find_b2 in Find_bb2. inv Find_bb2.
-            split; trivial.
-            destruct d. destruct Hb as [X1 [f1 [f2 [Hf1 Hf2]]]].
-                 destruct Hbb as [X2 [ff2 [f3 [Hff2 Hf3]]]].
-                  rewrite Hff2 in Hf2. inv Hf2.
-                 split. rewrite (EPC (Vptr b Int.zero) (Vptr b Int.zero) s). exists  (Vptr b Int.zero). split; assumption.
-                 exists f1. exists f3. split; assumption.
-         destruct Hb as [v1 [v2 [Hv1 [Hv2 GV12]]]].
-           destruct Hbb as [vv2 [v3 [Hvv2 [Hv3 GV23]]]].
-           rewrite Hvv2 in Hv2. inv Hv2.
-           exists v1. exists v3. split; trivial. split; trivial.
-             destruct v1; simpl in *.
-              destruct v2; simpl in *.
-                destruct v3; simpl in *. 
-                destruct GV12 as [? [? ?]].
-                rewrite  H. rewrite H0. rewrite H1. assumption.
-         destruct SimEq12 as [core_data12 match_core12 core_ord12 core_ord_wf12 core_diagram12 core_initial12 core_halted12 core_at_external12 core_after_external12].  
-          destruct SimExt23 as [core_data23 match_core23 core_ord23 core_ord_wf23 core_diagram23 core_initial23 core_halted23 core_at_external23 core_after_external23].
-           eapply Sim_ext.Build_Forward_simulation_extends with
-                 (core_data:= prod core_data12 core_data23)
-                 (match_state := fun d c1 m1 c3 m3 => match d with (d1,d2) => exists c2, match_core12 d1 c1 c2 /\ match_core23 d2 c2 m1 c3 m3 end).
-             eapply wf_lex_ord. apply core_ord_wf12. apply core_ord_wf23.
-             admit. (*core_diagram
-             intros c1 m1 c1' m1' CS1 [d12 d23] c3 [c2 [MC12 MC23]].
-                 destruct (core_diagram12 _ _ _ _ CS1 _ _ MC12) as [c2' [d12' [MC12' X]]].
-                 destruct X as [CS2 | CS2 ord12'].
-                     destruct (core_diagram23 _ _ _ _ H3*)
-             (*initial_core*)
-                  intros. rename v2 into v3. rewrite (EPC v1 v3 sig) in H. destruct H as [v2 [EP12 EP23]].
-                  assert (HT: Forall2 Val.has_type vals (sig_args sig)). eapply forall_lessdef_hastype; eauto.
-                  destruct (core_initial12 _ _ _ EP12 _ HT) as [d12 [c1 [c2 [Ini1 [Ini2 MC12]]]]].
-                  destruct (core_initial23 _ _ _ EP23 _ _ _ _ H0 H1 H2) as [d23 [c22 [c3 [Ini22 [Ini3 MC23]]]]].
-                  rewrite Ini22 in Ini2. inv Ini2.
-                  exists (d12,d23). exists c1. exists c3. split; trivial. split; trivial. exists c2. split; trivial.
-             (*safely_halted*)
-                    intros. rename st2 into c3. destruct cd as [d12 d23]. destruct H as [c2 [MC12 MC23]].
-                    apply (core_halted12 _ _ _ _ MC12) in H0.
-                    apply (core_halted23 _ _ _ _ _ _ MC23) in H0. assumption.
-             (*atexternal*)
-                    intros. rename st2 into st3. destruct cd as [d12 d23]. destruct H as [st2 [MC12 MC23]].
-                    apply (core_at_external12 _ _ _ _ _ _ MC12) in H0. destruct H0.
-                    apply (core_at_external23 _ _ _ _ _ _ _ _ MC23) in H. assumption.  
-             (*after_external*)
-                    intros. rename st2 into st3. destruct cd as [d12 d23]. destruct H as [st2 [MC12 MC23]].
-                    destruct (core_at_external12 _ _ _ _ _ _ MC12 H0)  as [AtExt2 _].
-                    assert (HVals1:  Forall2 Val.has_type vals1 (sig_args ef_sig)). eapply forall_lessdef_hastype; eauto.
-                    assert (HRet1:   Val.has_type ret1 (proj_sig_res ef_sig)). eapply lessdef_hastype; eauto.
-                    destruct (core_after_external12 _ _ _ _ _ _ _ MC12 H0 AtExt2 HVals1 HRet1) as [c1' [c2' [d12' [AftExt1 [AftExt2 MS12']]]]].
-                    destruct (core_after_external23 _ _ _ _ _ _ _ _ _ _ _ _ _ MC23 AtExt2 H1 H2 H3 H4 H5 H6 H7 H8 H9) as [c22' [c3' [d23' [AftExt22 [AftExt3 MS23']]]]].
-                    rewrite AftExt22 in AftExt2. inv AftExt2.
-                    exists c1'. exists c3'. exists (d12',d23'). split; trivial. split; trivial. exists c2'. split; trivial.
-             (*prog_main*)
-                   rewrite e12; assumption.
-             (*GenvHyp*) 
-                   destruct g23 as [Hyp2A Hyp2B].
-                   split; intros. rewrite Hyp2A. apply g12. 
-                                        rewrite Hyp2B. apply g12.
-     (*injection pass Sem2 -> Sem3*) 
-        rename C2 into C3. rename V2 into V3. rename F2 into F3. rename P2 into P3. rename Sem2 into Sem3.
-        rename C0 into C2. rename V0 into V2. rename F0 into F2. rename P0 into P2. rename Sem0 into Sem2.
-        clear H1 H3. rename Inj_init into Inj_init23. rename e into e23. rename g into g23. rename R into SimInj23.
-                               rename H0 into Extern1. rename H2 into Extern2. rename ePts_ok into ePts23_ok. rename H into EPC.
-                                rename i into i2. rename i0 into i3.
-       apply CompilerCorrectness.ccs_inj with (entrypoints:=entrypoints13)(jInit:=jInit); try assumption.
-         intros m Ini1.
-           destruct (Eq_init12 _ Ini1) as [m2 [Ini2 XX]]. subst.
-           apply (Inj_init23 _ Ini2).
+Qed.
+
+Lemma ePts_compose2: forall {F1 V1 F2 V2 F3 V3} 
+     (P1 : AST.program F1 V1) (P2 : AST.program F2 V2)  (P3 : AST.program F3 V3)
+     Epts12 Epts23 ExternIdents entrypoints13 jInit
+    (EPC : entrypoints_compose Epts12 Epts23 entrypoints13)
+    (ePts12_ok : CompilerCorrectness.entryPts_ok P1 P2 ExternIdents Epts12)
+    (ePts23_ok : CompilerCorrectness.entryPts_inject_ok P2 P3 jInit ExternIdents Epts23),
+    CompilerCorrectness.entryPts_inject_ok P1 P3 jInit ExternIdents entrypoints13.
+Proof. intros.
          unfold CompilerCorrectness.entryPts_inject_ok; intros e d EXT.
             destruct (ePts12_ok _ _ EXT) as [b1 [Find_b1 [Find_bb2 Hb]]].
             destruct (ePts23_ok _ _ EXT) as [b2 [b3 [Find_b2 [Find_b3 [initB2 Hbb]]]]].
@@ -209,30 +96,726 @@ induction SIM23; intros; subst.
                 destruct v3; simpl in *. 
                 destruct GV12 as [? [? ?]].
                 rewrite  H. rewrite H0. rewrite H1. assumption.
-         admit. (*need to prove  meminj_preserves_globals (Genv.globalenv P1) jInit  from meminj_preserves_globals (Genv.globalenv P2) jInit*)
+Qed.
+
+Inductive sem_compose_ord_eq_eq {D12 D23:Type} (ord12: D12 -> D12 -> Prop) (ord23: D23 -> D23 -> Prop) 
+         (C2:Type):
+         (D12 * option C2 * D23) ->  (D12 * option C2 * D23) ->  Prop := 
+
+    | sem_compose_ord1 :
+        forall (d12 d12':D12) (c2:C2) (d23:D23),
+           ord12 d12 d12' -> sem_compose_ord_eq_eq ord12 ord23 C2 (d12,Some c2,d23) (d12',Some c2,d23)
+    | sem_compose_ord2 :
+        forall (d12 d12':D12) (c2 c2':C2) (d23 d23':D23),
+           ord23 d23 d23' -> sem_compose_ord_eq_eq ord12 ord23 C2 (d12,Some c2,d23) (d12',Some c2',d23').
+
+Lemma well_founded_sem_compose_ord_eq_eq: forall {D12 D23:Type}
+                 (ord12: D12 -> D12 -> Prop) (ord23: D23 -> D23 -> Prop)  (C2:Type)
+                 (WF12: well_founded ord12) (WF23: well_founded ord23),
+                well_founded (sem_compose_ord_eq_eq ord12 ord23 C2). 
+  Proof. 
+    intros. intro. destruct a as [[d12 c2] d23].
+    revert d12. 
+    destruct c2. 
+    2: constructor; intros. 2: inv H.
+(*    set (q := (d23,c)).
+    change d23 with (fst q). change c with (snd q). clearbody q.
+    clear d23.*)
+   revert c. 
+    induction d23 using (well_founded_induction WF23).
+    intros.
+(*    set (q' := (d12,c)).
+    change d12 with (fst q'). change c with (snd q').
+    clearbody q'. clear d12 c.*)
+    induction d12 using (well_founded_induction WF12).
+    constructor; intros. inv H1.
+    generalize (H0 d0). simpl. intros.
+    apply H1. auto. (* destruct q'; auto.*) 
+    generalize (H d1). 
+    intros. 
+    spec H1. auto. (* destruct q; auto.*)
+    apply H1. 
+  Qed.
+
+Section EQEQ.
+Lemma diagram_eqeq: forall
+(G1 C1 D1 : Type)
+(G2 C2 D2 : Type)
+(G3 C3 D3 : Type)
+(Sem1 : CoreSemantics G1 C1 mem D1)
+(Sem2 : CoreSemantics G2 C2 mem D2)
+(Sem3 : CoreSemantics G3 C3 mem D3)
+(core_data12 : Type)
+(match_core12 : core_data12 -> C1 -> C2 -> Prop)
+(core_ord12 : core_data12 -> core_data12 -> Prop)
+(Genv2 : G2)
+(Genv1 : G1)
+(core_diagram12 : forall (st1 : C1) (m : mem) (st1' : C1) (m' : mem),
+                 corestep Sem1 Genv1 st1 m st1' m' ->
+                 forall (d : core_data12) (st2 : C2),
+                 match_core12 d st1 st2 ->
+                 exists st2' : C2,
+                   exists d' : core_data12,
+                     match_core12 d' st1' st2' /\
+                     (corestep_plus Sem2 Genv2 st2 m st2' m' \/
+                      corestep_star Sem2 Genv2 st2 m st2' m' /\
+                      core_ord12 d' d))
+(core_data23 : Type)
+(match_core23 : core_data23 -> C2 -> C3 -> Prop)
+(core_ord23 : core_data23 -> core_data23 -> Prop)
+(Genv3 : G3)
+(core_diagram23 : forall (st1 : C2) (m : mem) (st1' : C2) (m' : mem),
+                 corestep Sem2 Genv2 st1 m st1' m' ->
+                 forall (d : core_data23) (st2 : C3),
+                 match_core23 d st1 st2 ->
+                 exists st2' : C3,
+                   exists d' : core_data23,
+                     match_core23 d' st1' st2' /\
+                     (corestep_plus Sem3 Genv3 st2 m st2' m' \/
+                      corestep_star Sem3 Genv3 st2 m st2' m' /\
+                      core_ord23 d' d))
+(c1 : C1)
+(m1 : mem)
+(c1' : C1)
+(m1' : mem)
+(CS1 : corestep Sem1 Genv1 c1 m1 c1' m1')
+(d12 : core_data12)
+(d23 : core_data23)
+(c3 : C3)
+(c2 : C2)
+(MC12 : match_core12 d12 c1 c2)
+(MC23 : match_core23 d23 c2 c3),
+exists st2' : C3,
+  exists d' : core_data12 * option C2 * core_data23,
+    (let (y, d2) := d' in
+     let (d1, X) := y in
+     exists c0 : C2,
+       X = Some c0 /\ match_core12 d1 c1' c0 /\ match_core23 d2 c0 st2') /\
+    (corestep_plus Sem3 Genv3 c3 m1 st2' m1' \/
+     corestep_star Sem3 Genv3 c3 m1 st2' m1' /\
+     clos_trans (core_data12 * option C2 * core_data23)
+       (sem_compose_ord_eq_eq core_ord12 core_ord23 C2) d'
+       (d12, Some c2, d23)).
+Proof. intros.   destruct (core_diagram12 _ _ _ _ CS1 _ _ MC12) as [c2' [d12' [MC12' Y]]].
+    assert (ZZ: corestep_plus Sem2 Genv2 c2 m1 c2' m1' \/  (c2,m1) = (c2',m1') /\ core_ord12 d12' d12).
+       destruct Y. auto.
+       destruct H.
+       destruct H. destruct x.
+       right. split; auto.
+       left. exists x; auto.
+     clear Y. destruct ZZ as [CS2 | CS2 ord12'].
+     (*case1*)
+    destruct CS2.
+    clear MC12 CS1.
+    revert d23 c2 m1 c2' m1' c3 MC23 MC12' H.
+    induction x; intros. 
+      (*base case*) simpl in H.
+          destruct H as [c3' [m3' [? ?]]].
+          inv H0.
+          destruct (core_diagram23 _ _ _ _ H _ _ MC23) as [c3' [d23' [? ?]]].
+          exists c3'. exists (d12',Some c2',d23').
+          split. exists c2'. split. trivial. split; assumption. 
+          destruct H1. left; assumption.
+          destruct H1. right. split; trivial.
+          apply t_step. constructor 2. apply H2.
+     (*inductive case*)
+           remember (S x) as x'. simpl in H.
+           destruct H as [c2'' [m2'' [? ?]]]. subst x'.
+           destruct (core_diagram23 c2 m1 c2'' m2'' H _ _ MC23) as [c3' [d'' [? ?]]].
+           specialize (IHx _ _ _ _ _ _ H1 MC12' H0).
+           destruct IHx as [c3'' [d''' [? ?]]].
+           exists c3''. exists d'''.
+           split; auto.
+           (*inv H8. constructor. auto.
+           split. auto.*)
+           destruct H2; destruct H4.
+           (*1/4*)
+              left. destruct H2 as [n1 ?]. destruct H4 as [n2 ?].
+                      exists (n1 + S n2)%nat.
+                      change (S (n1 + S n2)) with (S n1 + S n2)%nat.
+                      rewrite corestepN_add. eauto.
+           (*2/4*)
+               destruct H4.
+               left. destruct H2 as [n1 ?]. destruct H4 as [n2 ?].
+                       exists (n1 + n2)%nat.
+                       change (S (n1 + n2)) with (S n1 + n2)%nat.
+                       rewrite corestepN_add. eauto.
+           (*3/4*)
+               left. destruct H2.
+                       destruct H2 as [n1 ?]. destruct H4 as [n2 ?].
+                       exists (n1 + n2)%nat.
+                       replace (S (n1 + n2)) with (n1 + S n2)%nat by omega.
+                       rewrite corestepN_add. eauto.
+           (*3/4*)
+               right. destruct H2. destruct H4.
+               split. destruct H2 as [n1 ?]. destruct H4 as [n2 ?].
+                         exists (n1 + n2)%nat.
+                         rewrite corestepN_add. eauto.
+              eapply t_trans; eauto.
+          (*4/4*)
+              apply t_step.
+              constructor 2. apply H5.
+  (*case 2*)
+    destruct CS2. inv H.
+    exists c3. exists (d12',Some c2',d23).
+    split. exists c2'.  split. trivial. split; assumption.
+(*    apply extends_refl.
+    inv H4.*)
+(*    split. constructor; auto.*)
+    right. split. exists O. simpl; auto.
+                       apply t_step. constructor 1; auto.
+Qed.
+
+Context {F1 C1 V1 F2 C2 V2 F3 C3 V3} 
+       (I :forall F C V : Type, CoreSemantics (Genv.t F V) C mem (list (ident * globvar V)) -> AST.program F V -> Prop)
+       (Sem1 : CoreSemantics (Genv.t F1 V1) C1 mem (list (ident * globvar V1)))
+       (Sem2 : CoreSemantics (Genv.t F2 V2) C2 mem (list (ident * globvar V2)))
+       (Sem3 : CoreSemantics (Genv.t F3 V3) C3 mem (list (ident * globvar V3)))
+       ExternIdents epts12  epts23 entrypoints13
+       (P1 : AST.program F1 V1) (P2 : AST.program F2 V2) (P3 : AST.program F3 V3) 
+       (ePts12_ok : CompilerCorrectness.entryPts_ok P1 P2 ExternIdents epts12)
+       (e12 : prog_main P1 = prog_main P2)
+       (g12: CompilerCorrectness.GenvHyp P1 P2)       
+       (EPC: entrypoints_compose epts12 epts23 entrypoints13)
+       (EXT1: In (prog_main P1, CompilerCorrectness.extern_func main_sig) ExternIdents)
+       (EXT2: In (prog_main P2, CompilerCorrectness.extern_func main_sig) ExternIdents)
+       (i1: I F1 C1 V1 Sem1 P1)
+       (Eq_init12 : forall m1 : mem,
+            initial_mem Sem1 (Genv.globalenv P1) m1 (prog_vars P1) ->
+            exists m2 : mem, initial_mem Sem2 (Genv.globalenv P2) m2 (prog_vars P2) /\ m1 = m2)
+       (SimEq12 : Sim_eq.Forward_simulation_equals mem (list (ident * globvar V1))
+                                          (list (ident * globvar V2)) Sem1 Sem2 (Genv.globalenv P1)
+                                          (Genv.globalenv P2) epts12) 
+       (SimEq23 : Sim_eq.Forward_simulation_equals mem (list (ident * globvar V2))
+                                         (list (ident * globvar V3)) Sem2 Sem3 (Genv.globalenv P2)
+                                         (Genv.globalenv P3) epts23) .
+(*
+Let D12:Type:= Sim_eq.core_data SimEq12.
+Let D23:Type:= Sim_eq.core_data SimEq23.
+
+  Let data13 := (Sim_eq.core_data SimEq12 * (option C2) * Sim_eq.core_data SimEq23)%type.
+
+  Inductive sem_compose_ord 
+      : (*data13 -> data13 -> Prop :=*)
+ (prod (prod (Sim_eq.core_data SimEq12) (option C2)) (Sim_eq.core_data SimEq23)) ->
+ (prod (prod (Sim_eq.core_data SimEq12) (option C2)) (Sim_eq.core_data SimEq23)) -> Prop :=
+
+    | sem_compose_ord1 :
+        forall (d12 d12':Sim_eq.core_data SimEq12) (c2:C2) (d23:Sim_eq.core_data SimEq23),
+           Sim_eq.core_ord SimEq12  d12 d12' ->
+           sem_compose_ord (d12,Some c2,d23) (d12',Some c2,d23)
+    | sem_compose_ord2 :
+        forall (d12 d12':Sim_eq.core_data SimEq12) (c2 c2':C2) (d23 d23':Sim_eq.core_data SimEq23),
+           Sim_eq.core_ord  SimEq23 d23 d23' ->
+           sem_compose_ord (d12,Some c2,d23) (d12',Some c2',d23').
+ 
+  Lemma well_founded_sem_compose_ord: well_founded sem_compose_ord. 
+  Proof. 
+    intro. destruct a as [[d12 c2] d23].
+    revert d12. 
+    destruct c2. 
+    2: constructor; intros. 2: inv H.
+(*    set (q := (d23,c)).
+    change d23 with (fst q). change c with (snd q). clearbody q.
+    clear d23.*)
+   revert c. 
+    induction d23 using (well_founded_induction (Sim_eq.core_ord_wf SimEq23)).
+    intros.
+(*    set (q' := (d12,c)).
+    change d12 with (fst q'). change c with (snd q').
+    clearbody q'. clear d12 c.*)
+    induction d12 using (well_founded_induction (Sim_eq.core_ord_wf SimEq12)).
+    constructor; intros. inv H1.
+    generalize (H0 d0). simpl. intros.
+    apply H1. auto. (* destruct q'; auto.*) 
+    generalize (H d1). 
+    intros. 
+    spec H1. auto. (* destruct q; auto.*)
+    apply H1. 
+  Qed.
+*)
+(*
+  Lemma well_founded_sem_compose_ord_withmem : well_founded sem_compose_ord.
+  Proof.
+    intro. destruct a as [[d12 [c2 m]] d23].
+    revert d12 m.
+    destruct c2.
+    2: constructor; intros. 2: inv H.
+(*    set (q := (d23,c)).
+    change d23 with (fst q). change c with (snd q). clearbody q.
+    clear d23 c.*)
+   revert c.
+    induction d23 using (well_founded_induction (Sim_eq.core_ord_wf SimEq23)).
+    intros.
+(*    set (q' := (d12,c)).
+    change d12 with (fst q'). change c with (snd q').
+    clearbody q'. clear d12 c.*)
+    induction d12 using (well_founded_induction (Sim_eq.core_ord_wf SimEq12)).
+    constructor; intros. inv H1.
+    generalize (H0 d12). simpl. intros.
+    apply H1. auto. (* destruct q'; auto.*)
+    generalize (H d23).
+    intros.
+    spec H1. auto. (* destruct q; auto.*)
+    apply H1.
+  Qed.
+*)
+
+Lemma eqeq: Sim_eq.Forward_simulation_equals mem (list (ident * globvar V1))
+                                       (list (ident * globvar V3)) Sem1 Sem3 (Genv.globalenv P1)
+                                       (Genv.globalenv P3) entrypoints13.
+Proof.
          destruct SimEq12 as [core_data12 match_core12 core_ord12 core_ord_wf12 core_diagram12 core_initial12 core_halted12 core_at_external12 core_after_external12].  
+         destruct SimEq23 as [core_data23 match_core23 core_ord23 core_ord_wf23 core_diagram23 core_initial23 core_halted23 core_at_external23 core_after_external23].
+          eapply Sim_eq.Build_Forward_simulation_equals with
+                 (core_data:= prod (prod core_data12 (option C2)) core_data23) 
+                 (match_core := fun d c1 c3 => match d with (d1,X,d2) => exists c2, X=Some c2 /\ match_core12 d1 c1 c2 /\ match_core23 d2 c2 c3 end)
+                 (core_ord := clos_trans _ (sem_compose_ord_eq_eq core_ord12 core_ord23 C2)).
+           (*wellfounded*) 
+                eapply wf_clos_trans. eapply well_founded_sem_compose_ord_eq_eq; assumption.
+           (*core_diagram*) 
+                 clear core_initial23  core_halted23 core_at_external23 core_after_external23 core_initial12  core_halted12 core_at_external12 core_after_external12 Eq_init12 SimEq12 SimEq23
+                          i1 I core_ord_wf23 core_ord_wf12 EXT2 EXT1 EPC e12 g12 ePts12_ok epts12  epts23 entrypoints13.
+                 intros. destruct d as [[d12 cc2] d23]. destruct H0 as [c2 [X [? ?]]]; subst.
+                 eapply (diagram_eqeq _ _ _ _ _ _ _ _ _ Sem1 Sem2 Sem3 core_data12 match_core12 _ _ _ core_diagram12 _ _ _ _ core_diagram23); eassumption. 
+           (*initial_core*)
+                  intros. rename v2 into v3. rewrite (EPC v1 v3 sig) in H. destruct H as [v2 [EP12 EP23]].
+                  destruct (core_initial12 _ _ _ EP12 _ H0) as [d12 [c1 [c2 [Ini1 [Ini2 MC12]]]]].
+                  destruct (core_initial23 _ _ _ EP23 _ H0) as [d23 [c22 [c3 [Ini22 [Ini3 MC23]]]]].
+                  rewrite Ini22 in Ini2. inv Ini2.
+                  exists (d12,Some c2,d23). exists c1. exists c3. split; trivial. split; trivial. exists c2. split; trivial. split; trivial.
+           (*safely_halted*)
+                    intros. rename c2 into c3. destruct cd as [[d12 cc2] d23]. destruct H as [c2 [X [MC12 MC23]]]. subst.
+                    apply (core_halted12 _ _ _ _ MC12) in H0.
+                    apply (core_halted23 _ _ _ _ MC23) in H0. assumption.
+           (*atexternal*)
+                    intros. rename st2 into st3. destruct d as [[d12cc2]  d23]. destruct H as [st2 [X [MC12 MC23]]]; subst.
+                    apply (core_at_external12 _ _ _ _ _ _ MC12) in H0. destruct H0.
+                    apply (core_at_external23 _ _ _ _ _ _ MC23) in H. assumption.  
+          (*after_external*)
+                    intros. rename st2 into st3. destruct d as [[d12 cc2] d23]. destruct H as [st2 [X [MC12 MC23]]]; subst.
+                    destruct (core_at_external12 _ _ _ _ _ _ MC12 H0)  as [AtExt2 _].
+                    destruct (core_after_external12 _ _ _ _ _ _ _ MC12 H0 AtExt2 H2 H3) as [c1' [c2' [d12' [AftExt1 [AftExt2 MS12']]]]].
+                    destruct (core_after_external23 _ _ _ _ _ _ _ MC23 AtExt2 H1 H2 H3) as [c22' [c3' [d23' [AftExt22 [AftExt3 MS23']]]]].
+                    rewrite AftExt22 in AftExt2. inv AftExt2.
+                    exists c1'. exists c3'. exists (d12',Some c2',d23'). split; trivial. split; trivial. exists c2'. split; trivial. split; trivial. 
+Qed.
+End EQEQ.
+
+Section EQEXT.
+Lemma diagram_eqext: forall
+(G1 C1 D1 : Type)
+(G2 C2 D2 : Type)
+(G3 C3 D3 : Type)
+(Sem1 : CoreSemantics G1 C1 mem D1)
+(Sem2 : CoreSemantics G2 C2 mem D2)
+(Sem3 : CoreSemantics G3 C3 mem D3)
+(core_data12 : Type)
+(match_core12 : core_data12 -> C1 -> C2 -> Prop)
+(core_ord12 : core_data12 -> core_data12 -> Prop)
+(Genv2 : G2)
+(Genv1 : G1)
+(core_diagram12 : forall (st1 : C1) (m : mem) (st1' : C1) (m' : mem),
+                 corestep Sem1 Genv1 st1 m st1' m' ->
+                 forall (d : core_data12) (st2 : C2),
+                 match_core12 d st1 st2 ->
+                 exists st2' : C2,
+                   exists d' : core_data12,
+                     match_core12 d' st1' st2' /\
+                     (corestep_plus Sem2 Genv2 st2 m st2' m' \/
+                      corestep_star Sem2 Genv2 st2 m st2' m' /\
+                      core_ord12 d' d))
+(core_data23 : Type)
+(match_core23 : core_data23 -> C2 -> mem -> C3 -> mem -> Prop)
+(core_ord23 : core_data23 -> core_data23 -> Prop)
+(Genv3 : G3)
+(core_diagram23 : forall (st1 : C2) (m1 : mem) (st1' : C2) (m1' : mem),
+                 corestep Sem2 Genv2 st1 m1 st1' m1' ->
+                 forall (cd : core_data23) (st2 : C3) (m2 : mem),
+                 match_core23 cd st1 m1 st2 m2 ->
+                 exists st2' : C3,
+                   exists m2' : mem,
+                     exists cd' : core_data23,
+                       match_core23 cd' st1' m1' st2' m2' /\
+                       (corestep_plus Sem3 Genv3 st2 m2 st2' m2' \/
+                        corestep_star Sem3 Genv3 st2 m2 st2' m2' /\ core_ord23 cd' cd))
+(st1 : C1)
+(m1 : mem)
+(st1' : C1)
+(m1' : mem)
+(CS1 : corestep Sem1 Genv1 st1 m1 st1' m1')
+(d12 : core_data12)
+(d23 : core_data23)
+(st3 : C3)
+(m3 : mem)
+(st2 : C2)
+(MC12: match_core12 d12 st1 st2)
+(MC23: match_core23 d23 st2 m1 st3 m3),
+exists st2' : C3,
+  exists m2' : mem,
+    exists cd' : core_data12 * option C2 * core_data23,
+      (let (y, d2) := cd' in
+       let (d1, X) := y in
+       exists c2 : C2,
+         X = Some c2 /\
+         match_core12 d1 st1' c2 /\ match_core23 d2 c2 m1' st2' m2') /\
+      (corestep_plus Sem3 Genv3 st3 m3 st2' m2' \/
+       corestep_star Sem3 Genv3 st3 m3 st2' m2' /\
+       clos_trans (core_data12 * option C2 * core_data23)
+         (sem_compose_ord_eq_eq core_ord12 core_ord23 C2) cd'
+         (d12, Some st2, d23)).
+Proof. intros.   destruct (core_diagram12 _ _ _ _ CS1 _ _ MC12) as [st2' [d12' [MC12' Y]]].
+    assert (ZZ: corestep_plus Sem2 Genv2 st2 m1 st2' m1' \/  (st2,m1) = (st2',m1') /\ core_ord12 d12' d12).
+       destruct Y. auto.
+       destruct H.
+       destruct H. destruct x.
+       right. split; auto.
+       left. exists x; auto.
+    clear Y. destruct ZZ as [CS2 | CS2 ord12'].
+     (*case1*)
+    destruct CS2.
+    clear MC12 CS1.
+    revert d23 st2 m1 st2' m1' st3 m3 MC23 MC12' H.
+    induction x; intros. 
+      (*base case*) simpl in H.
+          destruct H as [st3' [m3' [? ?]]].
+          inv H0.
+          destruct (core_diagram23 _ _ _ _ H _ _ _ MC23) as [st3' [m3' [d23' [? ?]]]].
+          exists st3'. exists m3'. exists (d12',Some st2',d23').
+          split. exists st2'. split. trivial. split; assumption. 
+          destruct H1. left; assumption.
+          destruct H1. right. split; trivial.
+          apply t_step. constructor 2. apply H2.
+     (*inductive case*)
+           remember (S x) as x'. simpl in H.
+           destruct H as [st2'' [m2'' [? ?]]]. subst x'.
+           destruct (core_diagram23 st2 m1 st2'' m2'' H _ _ _ MC23) as [c3' [m3' [d'' [? ?]]]].
+           specialize (IHx _ _ _ _ _ _ _ H1 MC12' H0).
+           destruct IHx as [c3'' [m3'' [[[d12''' cc2''] d23'']  [[c2'' [X [MC12'' MC23'']]] ?]]]]. subst.
+           exists c3''. exists m3''. exists (d12''', Some c2'',d23'').
+           split. exists c2''. auto.
+           (*inv H8. constructor. auto.
+           split. auto.*)
+           destruct H2; destruct H3.
+           (*1/4*)
+              left. destruct H2 as [n1 ?]. destruct H3 as [n2 ?].
+                      exists (n1 + S n2)%nat.
+                      change (S (n1 + S n2)) with (S n1 + S n2)%nat.
+                      rewrite corestepN_add. eauto.
+           (*2/4*)
+               destruct H3.
+               left. destruct H2 as [n1 ?]. destruct H3 as [n2 ?].
+                       exists (n1 + n2)%nat.
+                       change (S (n1 + n2)) with (S n1 + n2)%nat.
+                       rewrite corestepN_add. eauto.
+           (*3/4*)
+               left. destruct H2.
+                       destruct H2 as [n1 ?]. destruct H3 as [n2 ?].
+                       exists (n1 + n2)%nat.
+                       replace (S (n1 + n2)) with (n1 + S n2)%nat by omega.
+                       rewrite corestepN_add. eauto.
+           (*3/4*)
+               right. destruct H2. destruct H3.
+               split. destruct H2 as [n1 ?]. destruct H3 as [n2 ?].
+                         exists (n1 + n2)%nat.
+                         rewrite corestepN_add. eauto.
+              eapply t_trans; eauto.
+          (*4/4*)
+              apply t_step.
+              constructor 2. apply H4.
+  (*case 2*)
+    destruct CS2. inv H.
+    exists st3. exists m3. exists (d12',Some st2',d23).
+    split. exists st2'.  split. trivial. split; assumption.
+(*    apply extends_refl.
+    inv H4.*)
+(*    split. constructor; auto.*)
+    right. split. exists O. simpl; auto.
+                       apply t_step. constructor 1; auto.
+Qed.
+
+Context {F1 C1 V1 F2 C2 V2 F3 C3 V3} 
+       (I :forall F C V : Type, CoreSemantics (Genv.t F V) C mem (list (ident * globvar V)) -> AST.program F V -> Prop)
+       (Sem1 : CoreSemantics (Genv.t F1 V1) C1 mem (list (ident * globvar V1)))
+       (Sem2 : CoreSemantics (Genv.t F2 V2) C2 mem (list (ident * globvar V2)))
+       (Sem3 : CoreSemantics (Genv.t F3 V3) C3 mem (list (ident * globvar V3)))
+       ExternIdents epts12  epts23 entrypoints13
+       (P1 : AST.program F1 V1) (P2 : AST.program F2 V2) (P3 : AST.program F3 V3) 
+       (ePts12_ok : CompilerCorrectness.entryPts_ok P1 P2 ExternIdents epts12)
+       (e12 : prog_main P1 = prog_main P2)
+       (g12: CompilerCorrectness.GenvHyp P1 P2)       
+       (EPC: entrypoints_compose epts12 epts23 entrypoints13)
+       (EXT1: In (prog_main P1, CompilerCorrectness.extern_func main_sig) ExternIdents)
+       (EXT2: In (prog_main P2, CompilerCorrectness.extern_func main_sig) ExternIdents)
+       (i1: I F1 C1 V1 Sem1 P1)
+       (Eq_init12 : forall m1 : mem,
+            initial_mem Sem1 (Genv.globalenv P1) m1 (prog_vars P1) ->
+            exists m2 : mem, initial_mem Sem2 (Genv.globalenv P2) m2 (prog_vars P2) /\ m1 = m2)
+       (SimEq12 : Sim_eq.Forward_simulation_equals mem (list (ident * globvar V1))
+                                          (list (ident * globvar V2)) Sem1 Sem2 (Genv.globalenv P1)
+                                          (Genv.globalenv P2) epts12) 
+       (SimExt23 : Sim_ext.Forward_simulation_extends (list (ident * globvar V2))
+                            (list (ident * globvar V3)) Sem2 Sem3 (Genv.globalenv P2)
+                            (Genv.globalenv P3) epts23).
+
+Lemma eqext: Sim_ext.Forward_simulation_extends (list (ident * globvar V1))
+                                           (list (ident * globvar V3)) Sem1 Sem3 (Genv.globalenv P1)
+                                           (Genv.globalenv P3) entrypoints13.
+Proof.
+         destruct SimEq12 as [core_data12 match_core12 core_ord12 core_ord_wf12 core_diagram12 core_initial12 core_halted12 core_at_external12 core_after_external12].  
+         destruct SimExt23 as [core_data23 match_core23 core_ord23 core_ord_wf23 core_diagram23 core_initial23 core_halted23 core_at_external23 core_after_external23].
+           eapply Sim_ext.Build_Forward_simulation_extends with
+                 (match_state := fun d c1 m1 c3 m3 => match d with (d1,X,d2) => exists c2, X = Some c2 /\ match_core12 d1 c1 c2 /\ match_core23 d2 c2 m1 c3 m3 end)
+                 (core_data:= prod (prod core_data12 (option C2)) core_data23)
+                 (core_ord := clos_trans _ (sem_compose_ord_eq_eq core_ord12 core_ord23 C2)). 
+           (*well_founded*)
+                 eapply wf_clos_trans. eapply well_founded_sem_compose_ord_eq_eq; assumption.
+           (*core_diagram*) 
+                 clear core_initial23  core_halted23 core_at_external23 core_after_external23 core_initial12  core_halted12 core_at_external12 core_after_external12
+                          i1 I core_ord_wf23 core_ord_wf12 EXT2 EXT1 EPC e12 g12 ePts12_ok epts12  epts23 entrypoints13 Eq_init12 SimEq12 SimExt23.
+                 intros. rename st2 into st3.
+                 destruct cd as [[d12 cc2] d23]. destruct H0 as [st2 [X [? ?]]]; subst. rename m2 into m3.
+                 eapply (diagram_eqext _ _ _ _ _ _ _ _ _ Sem1 Sem2 Sem3 core_data12 match_core12 _ _ _ core_diagram12 _ _ _ _ core_diagram23); eassumption. 
+           (*initial_core*)
+                  intros. rename v2 into v3. rewrite (EPC v1 v3 sig) in H. destruct H as [v2 [EP12 EP23]].
+                  assert (HT: Forall2 Val.has_type vals (sig_args sig)). eapply forall_lessdef_hastype; eauto.
+                  destruct (core_initial12 _ _ _ EP12 _ HT) as [d12 [c1 [c2 [Ini1 [Ini2 MC12]]]]].
+                  destruct (core_initial23 _ _ _ EP23 _ _ _ _ H0 H1 H2) as [d23 [c22 [c3 [Ini22 [Ini3 MC23]]]]].
+                  rewrite Ini22 in Ini2. inv Ini2.
+                  exists (d12,Some c2,d23). exists c1. exists c3. split; trivial. split; trivial. exists c2. split; trivial. split; trivial.
+           (*safely_halted*)
+                    intros. rename st2 into c3. destruct cd as [[d12 cc2] d23]. destruct H as [c2 [X [MC12 MC23]]]; subst.
+                    apply (core_halted12 _ _ _ _ MC12) in H0.
+                    apply (core_halted23 _ _ _ _ _ _ MC23) in H0. assumption.
+           (*atexternal*)
+                    intros. rename st2 into st3. destruct cd as [[d12 cc2] d23]. destruct H as [st2 [X [MC12 MC23]]].
+                    apply (core_at_external12 _ _ _ _ _ _ MC12) in H0. destruct H0.
+                    apply (core_at_external23 _ _ _ _ _ _ _ _ MC23) in H. assumption.  
+           (*after_external*)
+                    intros. rename st2 into st3. destruct cd as [[d12 cc2] d23]. destruct H as [st2 [X [MC12 MC23]]].
+                    destruct (core_at_external12 _ _ _ _ _ _ MC12 H0)  as [AtExt2 _].
+                    assert (HVals1:  Forall2 Val.has_type vals1 (sig_args ef_sig)). eapply forall_lessdef_hastype; eauto.
+                    assert (HRet1:   Val.has_type ret1 (proj_sig_res ef_sig)). eapply lessdef_hastype; eauto.
+                    destruct (core_after_external12 _ _ _ _ _ _ _ MC12 H0 AtExt2 HVals1 HRet1) as [c1' [c2' [d12' [AftExt1 [AftExt2 MS12']]]]].
+                    destruct (core_after_external23 _ _ _ _ _ _ _ _ _ _ _ _ _ MC23 AtExt2 H1 H2 H3 H4 H5 H6 H7 H8 H9) as [c22' [c3' [d23' [AftExt22 [AftExt3 MS23']]]]].
+                    rewrite AftExt22 in AftExt2. inv AftExt2.
+                    exists c1'. exists c3'. exists (d12',Some c2',d23'). split; trivial. split; trivial. exists c2'. split; trivial. split; trivial.
+Qed.
+End EQEXT.
+
+Section EQINJ.
+Lemma diagram_eqinj: forall
+(G1 C1 D1 : Type)
+(G2 C2 D2 : Type)
+(G3 C3 D3 : Type)
+(Sem1 : CoreSemantics G1 C1 mem D1)
+(Sem2 : CoreSemantics G2 C2 mem D2)
+(Sem3 : CoreSemantics G3 C3 mem D3)
+(core_data12 : Type)
+(match_core12 : core_data12 -> C1 -> C2 -> Prop)
+(core_ord12 : core_data12 -> core_data12 -> Prop)
+(Genv2 : G2)
+(Genv1 : G1)
+(core_diagram12 : forall (st1 : C1) (m : mem) (st1' : C1) (m' : mem),
+                 corestep Sem1 Genv1 st1 m st1' m' ->
+                 forall (d : core_data12) (st2 : C2),
+                 match_core12 d st1 st2 ->
+                 exists st2' : C2,
+                   exists d' : core_data12,
+                     match_core12 d' st1' st2' /\
+                     (corestep_plus Sem2 Genv2 st2 m st2' m' \/
+                      corestep_star Sem2 Genv2 st2 m st2' m' /\
+                      core_ord12 d' d))
+(core_data23 : Type)
+(match_core23 : core_data23 -> meminj -> C2 -> mem -> C3 -> mem -> Prop)
+(core_ord23 : core_data23 -> core_data23 -> Prop)
+(Genv3 : G3) 
+(core_diagram23 : forall (st1 : C2) (m1 : mem) (st1' : C2) (m1' : mem),
+                 corestep Sem2 Genv2 st1 m1 st1' m1' ->
+                 forall (cd : core_data23) (st2 : C3) (j : meminj) (m2 : mem),
+                 match_core23 cd j st1 m1 st2 m2 ->
+                 exists st2' : C3,
+                   exists m2' : mem,
+                     exists cd' : core_data23,
+                       exists j' : meminj,
+                         inject_incr j j' /\
+                         inject_separated j j' m1 m2 /\
+                         match_core23 cd' j' st1' m1' st2' m2' /\
+                         (corestep_plus Sem3 Genv3 st2 m2 st2'
+                            m2' \/
+                          corestep_star Sem3 Genv3 st2 m2 st2'
+                            m2' /\ core_ord23 cd' cd))
+(st1 : C1)
+(m1 : mem)
+(st1' : C1)
+(m1' : mem)
+(CS1 : corestep Sem1 Genv1 st1 m1 st1' m1')
+(d12 : core_data12)
+(d23 : core_data23)
+(st3 : C3)
+(j : meminj)
+(m3 : mem)
+(st2 : C2)
+(MC12: match_core12 d12 st1 st2)
+(MC23: match_core23 d23 j st2 m1 st3 m3)
+(CSF2: corestep_fwd Sem2)
+(CSF3: corestep_fwd Sem3),
+exists st2' : C3,
+  exists m2' : mem,
+    exists cd' : core_data12 * option C2 * core_data23,
+      exists j' : meminj,
+        inject_incr j j' /\
+        inject_separated j j' m1 m3 /\
+        (let (y, d2) := cd' in
+         let (d1, X) := y in
+         exists c2 : C2,
+           X = Some c2 /\
+           match_core12 d1 st1' c2 /\ match_core23 d2 j' c2 m1' st2' m2') /\
+        (corestep_plus Sem3 Genv3 st3 m3 st2' m2' \/
+         corestep_star Sem3 Genv3 st3 m3 st2' m2' /\
+         clos_trans (core_data12 * option C2 * core_data23)
+           (sem_compose_ord_eq_eq core_ord12 core_ord23 C2) cd'
+           (d12, Some st2, d23)).
+Proof. intros.
+    destruct (core_diagram12 _ _ _ _ CS1 _ _ MC12) as [st2' [d12' [MC12' Y]]]. clear core_diagram12.
+    assert (ZZ: corestep_plus Sem2 Genv2 st2 m1 st2' m1' \/  (st2,m1) = (st2',m1') /\ core_ord12 d12' d12).
+       destruct Y. auto.
+       destruct H.
+       destruct H. destruct x.
+       right. split; auto.
+       left. exists x; auto.
+    clear Y. destruct ZZ as [CS2 | CS2 ord12'].
+     (*case1*) rename m1 into m2. rename m1' into m2'.
+    destruct CS2.
+    clear MC12 CS1.
+    revert j d23 st2 m2 st2' m2' st3 m3 MC23 MC12' H.
+    induction x; intros. 
+      (*base case*) simpl in H.
+          destruct H as [st3' [m3' [? ?]]].
+          inv H0.
+          destruct (core_diagram23 _ _ _ _ H _ _ _ _ MC23) as [st3' [m3' [d23' [j' [InjInc [InjSep [? ?]]]]]]].
+          exists st3'. exists m3'. exists (d12',Some st2',d23'). exists j'.
+          split; trivial.
+          split; trivial.
+          split. exists st2'. split. trivial. split; assumption. 
+          destruct H1. left; assumption.
+          destruct H1. right. split; trivial.
+          apply t_step. constructor 2. apply H2.
+     (*inductive case*)
+           remember (S x) as x'. simpl in H.
+           destruct H as [st2'' [m2'' [? ?]]]. subst x'.
+           destruct (core_diagram23 st2 m2 st2'' m2'' H _ _ _ _ MC23) as [c3' [m3' [d'' [j' [InjInc [InjSep [? ?]]]]]]].
+           specialize (IHx _ _ _ _ _ _ _ _ H1 MC12' H0).
+           destruct IHx as [c3'' [m3'' [[[d12''' cc2''] d23'']  [j'' [IncIncr' [InSep' [[c2'' [X [MC12'' MC23'']]] ?]]]]]]]. subst.
+           exists c3''. exists m3''. exists (d12''', Some c2'',d23''). exists j''.
+           split. eapply inject_incr_trans; eassumption.
+           split. apply CSF2 in H.
+                 intros b; intros.
+                 remember (j' b).
+                 destruct o; apply eq_sym in Heqo.
+                      destruct p. destruct (InjSep _ _ _ H4 Heqo). apply (IncIncr') in Heqo. rewrite Heqo in H5.  inv H5.  split; trivial.
+                 destruct (InSep' _ _ _ Heqo H5). split.
+                    intros N. apply H6. apply H. apply N.
+                    intros N. apply H7. 
+                        assert (FWD: mem_forward m3 m3').
+                           destruct H2 as [X | [X _]]. eapply corestep_plus_fwd; eassumption.  eapply corestep_star_fwd; eassumption.
+                        apply FWD. apply N.
+           split. exists c2''. auto.
+           (*inv H8. constructor. auto.
+           split. auto.*)
+           destruct H2; destruct H3.
+           (*1/4*)
+              left. destruct H2 as [n1 ?]. destruct H3 as [n2 ?].
+                      exists (n1 + S n2)%nat.
+                      change (S (n1 + S n2)) with (S n1 + S n2)%nat.
+                      rewrite corestepN_add. eauto.
+           (*2/4*)
+               destruct H3.
+               left. destruct H2 as [n1 ?]. destruct H3 as [n2 ?].
+                       exists (n1 + n2)%nat.
+                       change (S (n1 + n2)) with (S n1 + n2)%nat.
+                       rewrite corestepN_add. eauto.
+           (*3/4*)
+               left. destruct H2.
+                       destruct H2 as [n1 ?]. destruct H3 as [n2 ?].
+                       exists (n1 + n2)%nat.
+                       replace (S (n1 + n2)) with (n1 + S n2)%nat by omega.
+                       rewrite corestepN_add. eauto.
+           (*3/4*)
+               right. destruct H2. destruct H3.
+               split. destruct H2 as [n1 ?]. destruct H3 as [n2 ?].
+                         exists (n1 + n2)%nat.
+                         rewrite corestepN_add. eauto.
+              eapply t_trans; eauto.
+          (*4/4*)
+              apply t_step.
+              constructor 2. apply H4.
+  (*case 2*)
+    destruct CS2. inv H.
+    exists st3. exists m3. exists (d12',Some st2',d23). exists j.
+    split. apply inject_incr_refl.
+    split. apply inject_separated_same_meminj. 
+    split. exists st2'.  split. trivial. split; assumption.
+(*    apply extends_refl.
+    inv H4.*)
+(*    split. constructor; auto.*)
+    right. split. exists O. simpl; auto.
+                       apply t_step. constructor 1; auto.
+Qed.
+
+Context {F1 C1 V1 F2 C2 V2 F3 C3 V3} 
+       (I :forall F C V : Type, CoreSemantics (Genv.t F V) C mem (list (ident * globvar V)) -> AST.program F V -> Prop)
+       (Sem1 : CoreSemantics (Genv.t F1 V1) C1 mem (list (ident * globvar V1)))
+       (Sem2 : CoreSemantics (Genv.t F2 V2) C2 mem (list (ident * globvar V2)))
+       (Sem3 : CoreSemantics (Genv.t F3 V3) C3 mem (list (ident * globvar V3)))
+       ExternIdents epts12  epts23 entrypoints13
+       (P1 : AST.program F1 V1) (P2 : AST.program F2 V2) (P3 : AST.program F3 V3) 
+       (ePts12_ok : CompilerCorrectness.entryPts_ok P1 P2 ExternIdents epts12)
+       (e12 : prog_main P1 = prog_main P2)
+       (g12: CompilerCorrectness.GenvHyp P1 P2)       
+       (EPC: entrypoints_compose epts12 epts23 entrypoints13)
+       (EXT1: In (prog_main P1, CompilerCorrectness.extern_func main_sig) ExternIdents)
+       (EXT2: In (prog_main P2, CompilerCorrectness.extern_func main_sig) ExternIdents)
+       (i1: I F1 C1 V1 Sem1 P1)
+       (Eq_init12 : forall m1 : mem,
+            initial_mem Sem1 (Genv.globalenv P1) m1 (prog_vars P1) ->
+            exists m2 : mem, initial_mem Sem2 (Genv.globalenv P2) m2 (prog_vars P2) /\ m1 = m2)
+       (SimEq12 : Sim_eq.Forward_simulation_equals mem (list (ident * globvar V1))
+                                          (list (ident * globvar V2)) Sem1 Sem2 (Genv.globalenv P1)
+                                          (Genv.globalenv P2) epts12)  (SimInj23 : Sim_inj.Forward_simulation_inject (list (ident * globvar V2))
+             (list (ident * globvar V3)) Sem2 Sem3 (Genv.globalenv P2)
+             (Genv.globalenv P3) epts23)
+       (Fwd2: corestep_fwd Sem2) (Fwd3: corestep_fwd Sem3).
+
+Lemma eqinj: Sim_inj.Forward_simulation_inject (list (ident * globvar V1))
+                                        (list (ident * globvar V3)) Sem1 Sem3 (Genv.globalenv P1)
+                                        (Genv.globalenv P3) entrypoints13.
+Proof.
+          destruct SimEq12 as [core_data12 match_core12 core_ord12 core_ord_wf12 core_diagram12 core_initial12 core_halted12 core_at_external12 core_after_external12].  
          destruct SimInj23 as [core_data23 match_core23 core_ord23 core_ord_wf23 core_diagram23 core_initial23 core_halted23 core_at_external23 core_after_external23].
-           eapply Sim_inj.Build_Forward_simulation_inject with
-                 (core_data:= prod core_data12 core_data23)
-                 (match_state := fun d j c1 m1 c3 m3 => match d with (d1,d2) => exists c2, match_core12 d1 c1 c2 /\ match_core23 d2 j c2 m1 c3 m3 end).
-             eapply wf_lex_ord. apply core_ord_wf12. apply core_ord_wf23.
-             admit. (*core_diagram
-             intros c1 m1 c1' m1' CS1 [d12 d23] c3 [c2 [MC12 MC23]].
-                 destruct (core_diagram12 _ _ _ _ CS1 _ _ MC12) as [c2' [d12' [MC12' X]]].
-                 destruct X as [CS2 | CS2 ord12'].
-                     destruct (core_diagram23 _ _ _ _ H3*)
-             (*initial_core*)
+          eapply Sim_inj.Build_Forward_simulation_inject with
+                 (core_ord := clos_trans _ (sem_compose_ord_eq_eq core_ord12 core_ord23 C2))
+                 (match_state := fun d j c1 m1 c3 m3 => match d with (d1,X,d2) => exists c2, X=Some c2 /\ match_core12 d1 c1 c2 /\ match_core23 d2 j c2 m1 c3 m3 end).
+            (*well_founded*)
+                 eapply wf_clos_trans. eapply well_founded_sem_compose_ord_eq_eq; assumption.
+            (*core_diagram*)
+                 clear core_initial23  core_halted23 core_at_external23 core_after_external23 core_initial12  core_halted12 core_at_external12 core_after_external12
+                          i1 I core_ord_wf23 core_ord_wf12 EXT2 EXT1 EPC e12 g12 ePts12_ok epts12  epts23 entrypoints13 Eq_init12 SimEq12 SimInj23.
+                 intros. rename st2 into st3.
+                 destruct cd as [[d12 cc2] d23]. destruct H0 as [st2 [X [? ?]]]; subst. rename m2 into m3.
+                 eapply (diagram_eqinj _ _ _ _ _ _ _ _ _ Sem1 Sem2 Sem3 core_data12 match_core12 _ _ _ core_diagram12 _ _ _ _ core_diagram23); try eassumption.
+            (*initial_core*)
                   intros. rename v2 into v3. rewrite (EPC v1 v3 sig) in H. destruct H as [v2 [EP12 EP23]].
                   assert (HT: Forall2 Val.has_type vals1 (sig_args sig)). eapply forall_valinject_hastype; eauto.
                   destruct (core_initial12 _ _ _ EP12 _ HT) as [d12 [c11 [c2 [Ini1 [Ini2 MC12]]]]]. rewrite Ini1 in H0. inv H0.
                   destruct (core_initial23 _ _ _ EP23 _ _ _ _ _ _  Ini2 H1 H2 H3) as [d23 [c3 [Ini3 MC23]]].
-                  exists (d12,d23). exists c3. split; trivial. exists c2. split; trivial.
+                  exists (d12,Some c2,d23). exists c3. split; trivial. exists c2. auto.
              (*safely_halted*)
-                    intros. rename c2 into c3. destruct cd as [d12 d23]. destruct H as [c2 [MC12 MC23]].
+                    intros. rename c2 into c3. destruct cd as [[d12 cc2] d23]. destruct H as [c2 [X [MC12 MC23]]]; subst.
                     apply (core_halted12 _ _ _ _ MC12) in H0.
                     apply (core_halted23 _ _ _ _ _ _ _ MC23) in H0. assumption.
              (*atexternal*)
-                    intros. rename st2 into st3. destruct cd as [d12 d23]. destruct H as [st2 [MC12 MC23]].
+                    intros. rename st2 into st3. destruct cd as [[d12 cc2] d23]. destruct H as [c2 [X [MC12 MC23]]]; subst. 
                     apply (core_at_external12 _ _ _ _ _ _ MC12) in H0. destruct H0.
                     apply (core_at_external23 _ _ _ _ _ _ _ _ _ MC23) in H. 
                     destruct H as [MInj12 [PG2 X]]. 
@@ -240,23 +823,114 @@ induction SIM23; intros; subst.
                     split; try assumption. 
                     admit. (*need to prove  meminj_preserves_globals (Genv.globalenv P1) j  from meminj_preserves_globals (Genv.globalenv P2) j for any j*)  
              (*after_external*)
-                    intros. rename st2 into st3. destruct cd as [d12 d23]. destruct H0 as [st2 [MC12 MC23]].
+                    intros. rename st2 into st3. destruct cd as [[d12 cc2] d23]. destruct H0 as [c2 [X [MC12 MC23]]]; subst.
                     destruct (core_at_external12 _ _ _ _ _ _ MC12 H1)  as [AtExt2 HVals1].
                     assert (HRet1:   Val.has_type ret1 (proj_sig_res ef_sig)). eapply valinject_hastype; eassumption.
                     destruct (core_after_external12 _ _ _ _ _ _ _ MC12 H1 AtExt2 HVals1 HRet1) as [c1' [c2' [d12' [AftExt1 [AftExt2 MS12']]]]].
                     assert (PG2: meminj_preserves_globals (Genv.globalenv P2) j). admit.
                     destruct (core_after_external23 _ _ _ _ _ _ _ _ _ _ _ _ _ _ H MC23 AtExt2 PG2 H3 H4 H5 H6 H7 H8 H9 H10 H11) as [d23' [c22' [c3' [AftExt22 [AftExt3 MS23']]]]].
                     rewrite AftExt22 in AftExt2. inv AftExt2.
-                    exists (d12',d23'). exists c1'. exists c3'. split; trivial. split; trivial. exists c2'. split; trivial.
-             (*prog_main*)
-                   rewrite e12; assumption.
-             (*GenvHyp*) 
+                    exists (d12',Some c2',d23'). exists c1'. exists c3'. split; trivial. split; trivial. exists c2'. auto.
+Qed.
+End EQINJ.
+
+Lemma cc_trans_CaseEq: forall {F1 C1 V1 F2 C2 V2 F3 C3 V3} 
+     (Sem1 : CoreSemantics (Genv.t F1 V1) C1 mem (list (ident * globvar V1)))
+     (Sem2 : CoreSemantics (Genv.t F2 V2) C2 mem (list (ident * globvar V2)))
+     (Sem3 : CoreSemantics (Genv.t F3 V3) C3 mem (list (ident * globvar V3)))
+     ExternIdents epts12 epts23 I 
+     (P1 : AST.program F1 V1) (P2 : AST.program F2 V2) (P3 : AST.program F3 V3)
+     (ePts12_ok : CompilerCorrectness.entryPts_ok P1 P2 ExternIdents epts12)
+     (e12 : prog_main P1 = prog_main P2)
+     (g12: CompilerCorrectness.GenvHyp P1 P2)
+     (Eq_init12 : forall m1 : mem,
+          initial_mem Sem1 (Genv.globalenv P1) m1 (prog_vars P1) ->
+          exists m2 : mem,
+            initial_mem Sem2 (Genv.globalenv P2) m2 (prog_vars P2) /\ m1 = m2)
+     (SimEq12 : Sim_eq.Forward_simulation_equals mem (list (ident * globvar V1))
+                                (list (ident * globvar V2)) Sem1 Sem2 (Genv.globalenv P1)
+                               (Genv.globalenv P2) epts12)
+     (SIM23 : CompilerCorrectness.cc_sim I ExternIdents epts23 F2 C2 V2 F3 C3 V3 Sem2 Sem3 P2 P3)
+     (i1: I F1 C1 V1 Sem1 P1)
+     (Fwd2: corestep_fwd Sem2) (Fwd3: corestep_fwd Sem3),
+forall entrypoints13 : list (val * val * signature),
+entrypoints_compose epts12 epts23 entrypoints13 ->
+In (prog_main P1, CompilerCorrectness.extern_func main_sig) ExternIdents ->
+In (prog_main P2, CompilerCorrectness.extern_func main_sig) ExternIdents ->
+CompilerCorrectness.cc_sim I ExternIdents entrypoints13 F1 C1 V1 F3 C3 V3
+  Sem1 Sem3 P1 P3.
+Proof. 
+intros F1 C1 V1 F2 C2 V2 F3 C3 V3 Sem1 Sem2 Sem3 ExternIdents epts12 epts23 I  
+          P1 P2 P3 ePts12_ok e12 g12 Eq_init12 SimEq12 SIM23 i1.
+induction SIM23; intros; subst.
+ (*equality pass Sem2 -> Sem3*)  
+        rename C2 into C3. rename V2 into V3. rename F2 into F3. rename P2 into P3. rename Sem2 into Sem3.
+        rename C0 into C2. rename V0 into V2. rename F0 into F2. rename P0 into P2. rename Sem0 into Sem2.
+        rename Eq_init into Eq_init23. rename e into e23. rename g into g23. rename R into SimEq23.
+                               rename H0 into Extern1. rename H1 into Extern2. rename ePts_ok into ePts23_ok.
+                               rename H into EPC. rename i into i2. rename i0 into i3.
+       apply CompilerCorrectness.ccs_eq with (entrypoints:=entrypoints13);try assumption.
+       (*init_mem*)
+         intros m1 Ini1.
+           destruct (Eq_init12 _ Ini1) as [m2 [Ini2 XX]]. subst.
+           apply (Eq_init23 _ Ini2). 
+       (*entrypoints_ok*)
+           apply ePts_compose1 with (Prg2:=P2)(Epts12:=epts12)(Epts23:=epts23); assumption.
+       (*sim_eqeq*)
+           eapply eqeq; try eassumption.
+       (*prog_main*)
+           rewrite e12; assumption.
+       (*GenvHyp*) 
                    destruct g23 as [Hyp2A Hyp2B].
                    split; intros. rewrite Hyp2A. apply g12. 
                                         rewrite Hyp2B. apply g12.
-             (*externvars*) admit. (*preservation of externvars by equality phases even if V1->V2 etc*)
+ (*extension pass Sem2 -> Sem3*) 
+        rename C2 into C3. rename V2 into V3. rename F2 into F3. rename P2 into P3. rename Sem2 into Sem3.
+        rename C0 into C2. rename V0 into V2. rename F0 into F2. rename P0 into P2. rename Sem0 into Sem2.
+        rename Extends_init into Ext_init23. rename e into e23. rename g into g23. rename R into SimExt23.
+                               rename H0 into Extern1. rename H1 into Extern2. rename ePts_ok into ePts23_ok.
+                               rename H into EPC. rename i into i2. rename i0 into i3.
+       apply CompilerCorrectness.ccs_ext with (entrypoints:=entrypoints13); try assumption.
+       (*init_mem*)
+         intros m1 Ini1.
+           destruct (Eq_init12 _ Ini1) as [m2 [Ini2 XX]]. subst.
+           apply (Ext_init23 _ Ini2).
+       (*entrypoints_ok*)
+           apply ePts_compose1 with (Prg2:=P2)(Epts12:=epts12)(Epts23:=epts23); assumption.
+       (*sim_eqext*)  
+           eapply eqext; try eassumption.
+       (*prog_main*)
+           rewrite e12; assumption.
+       (*GenvHyp*) 
+                   destruct g23 as [Hyp2A Hyp2B].
+                   split; intros. rewrite Hyp2A. apply g12. 
+                                        rewrite Hyp2B. apply g12.
+   (*injection pass Sem2 -> Sem3*) 
+        rename C2 into C3. rename V2 into V3. rename F2 into F3. rename P2 into P3. rename Sem2 into Sem3.
+        rename C0 into C2. rename V0 into V2. rename F0 into F2. rename P0 into P2. rename Sem0 into Sem2.
+        rename Inj_init into Inj_init23. rename e into e23. rename g into g23. rename R into SimInj23.
+                               rename H0 into Extern1. rename H1 into Extern2. rename ePts_ok into ePts23_ok.
+                               rename H into EPC. rename i into i2. rename i0 into i3.
+       apply CompilerCorrectness.ccs_inj with (entrypoints:=entrypoints13)(jInit:=jInit); try assumption.
+       (*init_mem*)
+         intros m Ini1.
+           destruct (Eq_init12 _ Ini1) as [m2 [Ini2 XX]]. subst.
+           apply (Inj_init23 _ Ini2).
+       (*entrypoints_ok*)
+           eapply ePts_compose2; eassumption.
+       (*preserves_globals*) 
+         admit. (*need to prove  meminj_preserves_globals (Genv.globalenv P1) jInit  from meminj_preserves_globals (Genv.globalenv P2) jInit*)
+       (*sim_eqinj*) 
+           eapply eqinj; try eassumption.
+       (*prog_main*)
+             rewrite e12; assumption.
+       (*GenvHyp*) 
+             destruct g23 as [Hyp2A Hyp2B].
+             split; intros. rewrite Hyp2A. apply g12. 
+                                   rewrite Hyp2B. apply g12.
+       (*externvars*) intros b; intros. admit. (*preservation of externvars by equality phases even if V1->V2 etc*)
 Qed.
-
+      
 Lemma cc_trans_CaseExtends: forall {F1 C1 V1 F2 C2 V2 F3 C3 V3} 
      (Sem1 : CoreSemantics (Genv.t F1 V1) C1 mem (list (ident * globvar V1)))
      (Sem2 : CoreSemantics (Genv.t F2 V2) C2 mem (list (ident * globvar V2)))
@@ -275,15 +949,14 @@ Lemma cc_trans_CaseExtends: forall {F1 C1 V1 F2 C2 V2 F3 C3 V3}
                                 (list (ident * globvar V2)) Sem1 Sem2 (Genv.globalenv P1)
                               (Genv.globalenv P2) epts12)
      (SIM23 : CompilerCorrectness.cc_sim I ExternIdents epts23 F2 C2 V2 F3 C3 V3 Sem2 Sem3 P2 P3)
-     (i1: I F1 C1 V1 Sem1 P1),
+     (i1: I F1 C1 V1 Sem1 P1)
+     (*presumbaly, we'll need to add the fhe following assumptions in order to prove diagrm case of extends_inject:
+     (Fwd2: corestep_fwd Sem2) (Fwd3: corestep_fwd Sem3)*),
 forall entrypoints13 : list (val * val * signature),
-entrypoints_compose epts12 epts23 entrypoints13 ->
-In (prog_main P1, CompilerCorrectness.extern_func main_sig) ExternIdents ->
-prog_main P1 = prog_main P2 ->
-In (prog_main P2, CompilerCorrectness.extern_func main_sig) ExternIdents ->
-prog_main P2 = prog_main P3 ->
-CompilerCorrectness.cc_sim I ExternIdents entrypoints13 F1 C1 V1 F3 C3 V3
-  Sem1 Sem3 P1 P3.
+          entrypoints_compose epts12 epts23 entrypoints13 ->
+          In (prog_main P1, CompilerCorrectness.extern_func main_sig) ExternIdents ->
+          In (prog_main P2, CompilerCorrectness.extern_func main_sig) ExternIdents ->
+CompilerCorrectness.cc_sim I ExternIdents entrypoints13 F1 C1 V1 F3 C3 V3 Sem1 Sem3 P1 P3.
 Proof. 
 intros F1 C1 V1 F2 C2 V2 F3 C3 V3 Sem1 Sem2 Sem3 ExternIdents epts12 epts23 I  
           P1 P2 P3 ePts12_ok e12 g12 Ext_init12 SimExt12 SIM23 i1.
@@ -291,9 +964,9 @@ induction SIM23; intros; subst.
      (*equality pass Sem2 -> Sem3*) 
         rename C2 into C3. rename V2 into V3. rename F2 into F3. rename P2 into P3. rename Sem2 into Sem3.
         rename C0 into C2. rename V0 into V2. rename F0 into F2. rename P0 into P2.  rename Sem0 into Sem2.
-        clear H1 H3. rename Eq_init into Eq_init23. rename e into e23. rename g into g23. rename R into SimEq23.
-                               rename H0 into Extern1. rename H2 into Extern2. rename ePts_ok into ePts23_ok. rename H into EPC.
-                                rename i into i2. rename i0 into i3.
+        rename Eq_init into Eq_init23. rename e into e23. rename g into g23. rename R into SimEq23.
+                               rename H0 into Extern1. rename H1 into Extern2. rename ePts_ok into ePts23_ok.
+                               rename H into EPC. rename i into i2. rename i0 into i3.
        apply CompilerCorrectness.ccs_ext with (entrypoints:=entrypoints13); try assumption.
          intros m1 Ini1.
            destruct (Ext_init12 _ Ini1) as [m2 [Ini2 XX]].
@@ -361,9 +1034,9 @@ induction SIM23; intros; subst.
      (*extension pass Sem2 -> Sem3*) 
         rename C2 into C3. rename V2 into V3. rename F2 into F3. rename P2 into P3. rename Sem2 into Sem3.
         rename C0 into C2. rename V0 into V2. rename F0 into F2. rename P0 into P2.  rename Sem0 into Sem2.
-        clear H1 H3. rename Extends_init into Ext_init23. rename e into e23. rename g into g23. rename R into SimExt23.
-                               rename H0 into Extern1. rename H2 into Extern2. rename ePts_ok into ePts23_ok. rename H into EPC.
-                                rename i into i2. rename i0 into i3.
+        rename Extends_init into Ext_init23. rename e into e23. rename g into g23. rename R into SimExt23.
+                               rename H0 into Extern1. rename H1 into Extern2. rename ePts_ok into ePts23_ok. 
+                               rename H into EPC. rename i into i2. rename i0 into i3.
        apply CompilerCorrectness.ccs_ext with (entrypoints:=entrypoints13); try assumption.
          intros m1 Ini1.
            destruct (Ext_init12 _ Ini1) as [m2 [Ini2 MExt12]].
@@ -449,9 +1122,9 @@ induction SIM23; intros; subst.
      (*injection pass Sem2 -> Sem3*) 
         rename C2 into C3. rename V2 into V3. rename F2 into F3. rename P2 into P3.  rename Sem2 into Sem3.
         rename C0 into C2. rename V0 into V2. rename F0 into F2. rename P0 into P2. rename Sem0 into Sem2.
-        clear H1 H3. rename Inj_init into Inj_init23. rename e into e23. rename g into g23. rename R into SimInj23.
-                               rename H0 into Extern1. rename H2 into Extern2. rename ePts_ok into ePts23_ok. rename H into EPC.
-                                rename i into i2. rename i0 into i3.
+        rename Inj_init into Inj_init23. rename e into e23. rename g into g23. rename R into SimInj23.
+                               rename H0 into Extern1. rename H1 into Extern2. rename ePts_ok into ePts23_ok. 
+                               rename H into EPC. rename i into i2. rename i0 into i3.
        apply CompilerCorrectness.ccs_inj with (entrypoints:=entrypoints13)(jInit:=jInit); try assumption.
          intros m1 Ini1.
            destruct (Ext_init12 _ Ini1) as [m2 [Ini2 MExt12]]. 
@@ -543,7 +1216,6 @@ induction SIM23; intros; subst.
              (*externvars*) admit. (*preservation of externvars by extension phases even if V1->V2 etc*)
 Qed.
 
-
 Lemma val_inject_split: forall v1 v3 j1 j2 (V:val_inject (compose_meminj j1 j2) v1 v3),
          exists v2, val_inject j1 v1 v2 /\ val_inject j2 v2 v3.
 Proof. intros.
@@ -588,13 +1260,10 @@ Lemma cc_trans_CaseInject: forall {F1 C1 V1 F2 C2 V2 F3 C3 V3}
      (SIM23 : CompilerCorrectness.cc_sim I ExternIdents epts23 F2 C2 V2 F3 C3 V3 Sem2 Sem3 P2 P3)
      (i1: I F1 C1 V1 Sem1 P1),
 forall entrypoints13 : list (val * val * signature),
-entrypoints_compose epts12 epts23 entrypoints13 ->
-In (prog_main P1, CompilerCorrectness.extern_func main_sig) ExternIdents ->
-prog_main P1 = prog_main P2 ->
-In (prog_main P2, CompilerCorrectness.extern_func main_sig) ExternIdents ->
-prog_main P2 = prog_main P3 ->
-CompilerCorrectness.cc_sim I ExternIdents entrypoints13 F1 C1 V1 F3 C3 V3
-  Sem1 Sem3 P1 P3.
+           entrypoints_compose epts12 epts23 entrypoints13 ->
+            In (prog_main P1, CompilerCorrectness.extern_func main_sig) ExternIdents ->
+            In (prog_main P2, CompilerCorrectness.extern_func main_sig) ExternIdents ->
+CompilerCorrectness.cc_sim I ExternIdents entrypoints13 F1 C1 V1 F3 C3 V3 Sem1 Sem3 P1 P3.
 Proof.
 intros F1 C1 V1 F2 C2 V2 F3 C3 V3 Sem1 Sem2 Sem3 ExternIdents epts12 epts23 I  
           P1 P2 P3 e12 g12 VarsOK1 j12 ePts12_ok Inj_init12 PG1 SimInj12 SIM23 i1.
@@ -602,9 +1271,9 @@ induction SIM23; intros; subst.
      (*equality pass Sem2 -> Sem3*) 
         rename C2 into C3. rename V2 into V3. rename F2 into F3. rename P2 into P3. rename Sem2 into Sem3.
         rename C0 into C2. rename V0 into V2. rename F0 into F2. rename P0 into P2.  rename Sem0 into Sem2.
-        clear H1 H3. rename Eq_init into Eq_init23. rename e into e23. rename g into g23. rename R into SimEq23.
-                               rename H0 into Extern1. rename H2 into Extern2. rename ePts_ok into ePts23_ok. rename H into EPC.
-                                rename i into i2. rename i0 into i3.
+        rename Eq_init into Eq_init23. rename e into e23. rename g into g23. rename R into SimEq23.
+                               rename H0 into Extern1. rename H1 into Extern2. rename ePts_ok into ePts23_ok.
+                               rename H into EPC. rename i into i2. rename i0 into i3.
        apply CompilerCorrectness.ccs_inj with (entrypoints:=entrypoints13)(jInit:=j12); try assumption.
          intros m1 Ini1.
            destruct (Inj_init12 _ Ini1) as [m2 [Ini2 MInj12]].
@@ -630,8 +1299,7 @@ induction SIM23; intros; subst.
                 destruct GV12 as [? [? ?]].
                 rewrite  H. rewrite H0. rewrite H1. assumption.
          destruct SimInj12 as [core_data12 match_core12 core_ord12 core_ord_wf12 core_diagram12 core_initial12 core_halted12 core_at_external12 core_after_external12].  
-(*               assert (YY := @eq_simulation_star _ _ _ _ _ _ _ Sem2 Sem3 (Genv.globalenv P2)  (Genv.globalenv P3) entrypoints0).*)
-           destruct SimEq23 as [core_data23 match_core23 core_ord23 core_ord_wf23 core_diagram23 core_initial23 core_halted23 core_at_external23 core_after_external23].
+          destruct SimEq23 as [core_data23 match_core23 core_ord23 core_ord_wf23 core_diagram23 core_initial23 core_halted23 core_at_external23 core_after_external23].
            eapply Sim_inj.Build_Forward_simulation_inject with
                  (core_data:= prod core_data12 core_data23)
                  (match_state := fun d j c1 m1 c3 m3 => match d with (d1,d2) => exists c2, match_core12 d1 j c1 m1 c2 m3 /\ match_core23 d2 c2 c3 end).
@@ -676,9 +1344,9 @@ induction SIM23; intros; subst.
      (*extension pass Sem2 -> Sem3*) 
         rename C2 into C3. rename V2 into V3. rename F2 into F3. rename P2 into P3. rename Sem2 into Sem3.
         rename C0 into C2. rename V0 into V2. rename F0 into F2. rename P0 into P2.  rename Sem0 into Sem2.
-        clear H1 H3. rename Extends_init into Ext_init23. rename e into e23. rename g into g23. rename R into SimExt23.
-                               rename H0 into Extern1. rename H2 into Extern2. rename ePts_ok into ePts23_ok. rename H into EPC.
-                                rename i into i2. rename i0 into i3.
+        rename Extends_init into Ext_init23. rename e into e23. rename g into g23. rename R into SimExt23.
+                               rename H0 into Extern1. rename H1 into Extern2. rename ePts_ok into ePts23_ok. 
+                               rename H into EPC. rename i into i2. rename i0 into i3.
        apply CompilerCorrectness.ccs_inj with (entrypoints:=entrypoints13)(jInit:=j12); try assumption.
          intros m1 Ini1.
            destruct (Inj_init12 _ Ini1) as [m2 [Ini2 MIni12]].
@@ -707,7 +1375,7 @@ induction SIM23; intros; subst.
                 destruct GV12 as [? [? ?]].
                 rewrite  H. rewrite H0. rewrite H1. assumption.
          destruct SimInj12 as [core_data12 match_core12 core_ord12 core_ord_wf12 core_diagram12 core_initial12 core_halted12 core_at_external12 core_after_external12].  
-           destruct SimExt23 as [core_data23 match_core23 core_ord23 core_ord_wf23 core_diagram23 core_initial23 core_halted23 core_at_external23 core_after_external23].
+         destruct SimExt23 as [core_data23 match_core23 core_ord23 core_ord_wf23 core_diagram23 core_initial23 core_halted23 core_at_external23 core_after_external23].
            eapply Sim_inj.Build_Forward_simulation_inject with
                  (core_data:= prod core_data12 core_data23)
                  (match_state := fun d j c1 m1 c3 m3 => match d with (d1,d2) => exists c2, exists m2, match_core12 d1 j c1 m1 c2 m2 /\ match_core23 d2 c2 m2 c3 m3 end).
@@ -764,9 +1432,9 @@ induction SIM23; intros; subst.
      (*injection pass Sem2 -> Sem3*) 
         rename C2 into C3. rename V2 into V3. rename F2 into F3. rename P2 into P3.  rename Sem2 into Sem3.
         rename C0 into C2. rename V0 into V2. rename F0 into F2. rename P0 into P2. rename Sem0 into Sem2.
-        clear H1 H3. rename Inj_init into Inj_init23. rename e into e23. rename g into g23. rename R into SimInj23.
-                               rename H0 into Extern1. rename H2 into Extern2. rename ePts_ok into ePts23_ok. rename H into EPC.
-                                rename i into i2. rename i0 into i3. rename jInit into j23.
+        rename Inj_init into Inj_init23. rename e into e23. rename g into g23. rename R into SimInj23.
+                               rename H0 into Extern1. rename H1 into Extern2. rename ePts_ok into ePts23_ok.
+                               rename H into EPC. rename i into i2. rename i0 into i3. rename jInit into j23.
        apply CompilerCorrectness.ccs_inj with (entrypoints:=entrypoints13)(jInit:=compose_meminj j12 j23); try assumption.
          intros m1 Ini1.
            destruct (Inj_init12 _ Ini1) as [m2 [Ini2 Minj12]]. 
@@ -795,7 +1463,7 @@ induction SIM23; intros; subst.
                 rewrite  H. rewrite H0. rewrite H1. assumption.
          admit. (*need to prove  meminj_preserves_globals (Genv.globalenv P1) jInit  from meminj_preserves_globals (Genv.globalenv P2) jInit*)
          destruct SimInj12 as [core_data12 match_core12 core_ord12 core_ord_wf12 core_diagram12 core_initial12 core_halted12 core_at_external12 core_after_external12].  
-           destruct SimInj23 as [core_data23 match_core23 core_ord23 core_ord_wf23 core_diagram23 core_initial23 core_halted23 core_at_external23 core_after_external23].
+         destruct SimInj23 as [core_data23 match_core23 core_ord23 core_ord_wf23 core_diagram23 core_initial23 core_halted23 core_at_external23 core_after_external23].
            eapply Sim_inj.Build_Forward_simulation_inject with
                  (core_data:= prod core_data12 core_data23)
                  (match_state := fun d j c1 m1 c3 m3 => match d with (d1,d2) => exists c2, exists m2, exists j1, exists j2, j = compose_meminj j1 j2 /\
@@ -882,14 +1550,15 @@ Theorem cc_trans:
         F3 V3 C3
         (Sem3: CoreSemantics (Genv.t F3 V3) C3 mem (list (ident * globvar V3)))
         entrypoints23 P3 (SIM23:CompilerCorrectness.cc_sim I ExternIdents entrypoints23 F2 C2 V2 F3 C3 V3 Sem2 Sem3 P2 P3)
+        (Fwd2: corestep_fwd Sem2) (Fwd3: corestep_fwd Sem3)
        entrypoints13 (EPC:entrypoints_compose entrypoints12 entrypoints23 entrypoints13),
-        In (P1.(prog_main), CompilerCorrectness.extern_func main_sig) ExternIdents  -> P1.(prog_main) = P2.(prog_main) ->
-                 In (P2.(prog_main), CompilerCorrectness.extern_func main_sig) ExternIdents  -> P2.(prog_main) = P3.(prog_main) ->
-                 CompilerCorrectness.cc_sim I ExternIdents entrypoints13 F1 C1 V1 F3 C3 V3 Sem1 Sem3 P1 P3.
+        In (P1.(prog_main), CompilerCorrectness.extern_func main_sig) ExternIdents  -> 
+        In (P2.(prog_main), CompilerCorrectness.extern_func main_sig) ExternIdents  ->
+CompilerCorrectness.cc_sim I ExternIdents entrypoints13 F1 C1 V1 F3 C3 V3 Sem1 Sem3 P1 P3.
 Proof.
   intros  ExternIdents epts12 I F1 C1 V1 F2 C2 V2 Sem1 Sem2 P1 P2 SIM12.
-  induction SIM12; intros F3 V3 C3 Sem3 epts23 P3 SIM23.
-  eapply (cc_trans_CaseEq Sem1 Sem2 Sem3); assumption.
+  induction SIM12; intros F3 V3 C3 Sem3 epts23 P3 SIM23 Fwd2 Fwd3.
+  eapply (cc_trans_CaseEq Sem1 Sem2 Sem3); try assumption.
   eapply (cc_trans_CaseExtends Sem1 Sem2 Sem3); assumption.
   eapply (cc_trans_CaseInject Sem1 Sem2 Sem3) with (j12:=jInit); assumption.
 Qed.
